Adding support for prophecy variables to heap_lang

theories/heap_lang/adequacy.v
@@ -1,24 +1,27 @@
 From iris.program_logic Require Export weakestpre adequacy.
 From iris.algebra Require Import auth.
-From iris.heap_lang Require Import proofmode notation.
+From iris.heap_lang Require Import proofmode notation proph_map.
 From iris.proofmode Require Import tactics.
 Set Default Proof Using "Type".
 
-Class heapPreG Σ := HeapPreG {
-  heap_preG_iris :> invPreG Σ;
-  heap_preG_heap :> gen_heapPreG loc val Σ
+Class heap_prophPreG Σ := HeapProphPreG {
+  heap_proph_preG_iris :> invPreG Σ;
+  heap_proph_preG_heap :> gen_heapPreG loc val Σ;
+  heap_proph_preG_proph :> proph_mapPreG proph val Σ
 }.
 
-Definition heapΣ : gFunctors := #[invΣ; gen_heapΣ loc val].
-Instance subG_heapPreG {Σ} : subG heapΣ Σ → heapPreG Σ.
+Definition heapΣ : gFunctors := #[invΣ; gen_heapΣ loc val; proph_mapΣ proph val].
+Instance subG_heapPreG {Σ} : subG heapΣ Σ → heap_prophPreG Σ.
 Proof. solve_inG. Qed.
 
-Definition heap_adequacy Σ `{heapPreG Σ} s e σ φ :
+Definition heap_adequacy Σ `{heap_prophPreG Σ} s e σ φ :
   (∀ `{heapG Σ}, WP e @ s; ⊤ {{ v, ⌜φ v⌝ }}%I) →
   adequate s e σ (λ v _, φ v).
 Proof.
   intros Hwp; eapply (wp_adequacy _ _); iIntros (??) "".
-  iMod (gen_heap_init σ) as (?) "Hh".
-  iModIntro. iExists (fun σ _ => gen_heap_ctx σ). iFrame "Hh".
-  iApply (Hwp (HeapG _ _ _)).
+  iMod (gen_heap_init σ.1) as (?) "Hh".
+  iMod (proph_map_init κs σ.2) as (?) "Hp".
+  iModIntro.
+  iExists (fun σ κs => (gen_heap_ctx σ.1 ∗ proph_map_ctx κs σ.2)%I). iFrame.
+  iApply (Hwp (HeapG _ _ _ _)).
 Qed.
